theories/Syntax/Messages.v
@@ -39,6 +39,7 @@ From Katamaran Require Import
      Environment
      Notations
      Prelude
+     Symbolic.Instantiation
      Symbolic.OccursCheck
      Syntax.BinOps
      Syntax.Terms
@@ -57,6 +58,7 @@ Local Set Implicit Arguments.
 Module Type MessagesOn
   (Import TY : Types)
   (Import TM : TermsOn TY)
+  (Import IN : InstantiationOn TY TM)
   (Import OC : OccursCheckOn TY TM).
 
   Local Notation LCtx := (NCtx LVar Ty).
@@ -102,5 +104,35 @@ Module Type MessagesOn
   End amsg.
   Export amsg (AMessage).
   Export (hints) amsg.
+
+  Module wmsg.
+
+    Record WithMessage (A : LCtx -> Type) (Σ : LCtx) : Type :=
+      mk { msg : AMessage Σ; from : A Σ; }.
+    #[global] Arguments mk {A Σ} _ _.
+    #[global] Arguments wmsg.from {A Σ} _.
+
+    (* Use the same prioity that an instance of pairs would have. *)
+    #[export] Instance subst_wmessage `{Subst A} : Subst (WithMessage A) | 2 :=
+      fun _ '(mk m x) _ ζ => mk (subst m ζ) (subst x ζ).
+
+    (* Use the same prioity that an instance of pairs would have. *)
+    #[export] Instance substlaws_wmessage `{SubstLaws A} : SubstLaws (WithMessage A) | 2.
+    Proof.
+      constructor.
+      - intros ? []; cbn; f_equal; apply subst_sub_id.
+      - intros ? ? ? ? ? []; cbn; f_equal; apply subst_sub_comp.
+    Qed.
+
+    #[export] Instance inst_wmessage `{Inst A Prop} : Inst (WithMessage A) Prop :=
+      fun Σ '(mk _ x) ι => inst x ι.
+
+    #[export] Instance instsubst_wmessage `{InstSubst A Prop} :
+      InstSubst (WithMessage A) Prop :=
+      fun _ _ ζ ι '(mk _ x) => inst_subst ζ ι x.
+
+  End wmsg.
+  Export wmsg (WithMessage).
+  Export (hints) wmsg.
 
 End MessagesOn.
